proofs/option_derivative.v
@@ -1,0 +1,320 @@
+Load metaproperties.
+
+(* An option derivative *)
+Definition option_derivative (t period : Time) :=
+  (And
+     (Before t (Or (Give (One USD)) (Give (One EUR))))
+     (After (t + period) (Scale 2 (One EUR)))
+  ).
+
+
+(* The owners rights *)
+Lemma option_I_to_O_helper:
+  forall s1 s2 t T period I O sc ctr ctr_id dsc_id,
+    consistent_state s1 ->
+    ctr = finctr ctr_id dsc_id (After (t + period) (Scale 2 (One EUR))) I O O sc ->
+    joins O ctr s1 s2 T ->
+    T > t + period ->
+    O <> 0 ->
+    exists tr,
+      In tr (m_ledger s2) /\
+      tr_ctr_id tr = ctr_id /\
+      tr_from tr = I /\
+      tr_to tr = O /\
+      tr_amount tr = sc * 2.
+Proof.
+  intros.
+  destruct_join H1.
+  - insert_consistent s Ss.
+    induction St; subst s'.
+    + inversion_event Ev. find_contradiction H.
+    + ctr_case_analysis ctr ctr0.
+      execute_own ctr H10.
+      case_if H10.
+      case_if H13.
+      * eexists. split.
+        ** eapply steps_does_not_remove_transactions; eauto.
+           simpl. subst ledger'. left. eauto.
+        ** repeat split; trivial. resolve_owner H5.
+      * simpl in *. rewrite <- T0 in *.
+        apply ltb_sound_false in H10. contradiction H10.
+    + not_or ctr ctr0 H7.
+    + not_or ctr ctr0 H7.
+    + inversion_event Ev. find_contradiction H.
+    + find_contradiction H.
+  - insert_consistent s Ss.
+    induction St; subst s'.
+    + inversion_event Ev. find_contradiction_del H.
+    + inversion_event Ev. find_contradiction_del H.
+    + not_or ctr ctr0 H7.
+    + not_or ctr ctr0 H7.
+    + ctr_case_analysis ctr ctr0.
+      execute_own ctr H8.
+      case_if H8.
+      * apply ltb_sound_true in H0.
+        apply Nat.lt_asymm in H0.
+        contradict H0. apply infinite.
+      * case_if H11.
+    + find_contradiction_del H.
+Qed.
+
+Proposition option_I_to_O :
+  forall s1 s2 t T gen_ctr period I O sc ctr c_id dsc_id,
+    consistent_state s1 ->
+    ctr = finctr c_id dsc_id (option_derivative t period) I O O sc ->
+    joins_generated O ctr gen_ctr s1 s2 t T ->
+    (ctr_primitive gen_ctr) = After (t + period) (Scale 2 (One EUR)) ->
+    T > t + period ->
+    O <> 0 ->
+    exists tr,
+      In tr (m_ledger s2) /\
+      tr_ctr_id tr = (ctr_id gen_ctr) /\
+      tr_from tr = I /\
+      tr_to tr = O /\
+      tr_amount tr = sc * 2.
+Proof.
+  intros.
+  destruct_join_gen H1.
+  - insert_consistent s Ss.
+    insert_consistent s' St.
+    induction St; subst s'.
+    + inversion_event Ev. find_contradiction M.
+    + ctr_case_analysis ctr ctr0.
+      execute_own ctr H12.
+      case_analysis H12.
+      case_analysis H15.
+      * case_analysis H16.
+        case_analysis H17; simpl in *;
+          rewrite H0, H12, H14, H15 in Exec; inversion Exec; clear Exec;
+            rewrite <- H17 in M0; simpl in M0.
+        ** destruct M0 as [M0 | M0]; try contradiction.
+           rewrite <- M0 in H2. simpl in H2. inversion H2.
+        ** destruct M0 as [M0 | [M0 | M0]]; try contradiction.
+           *** rewrite <- M0 in H2. simpl in H2. inversion H2.
+           *** eapply option_I_to_O_helper; eauto.
+               rewrite <- M0 in J.
+               rewrite <- M0. simpl.               
+               exact J.
+      * case_analysis H16.
+        case_analysis H17; simpl in *;
+          rewrite H0, H12, H14, H15 in Exec; inversion Exec; clear Exec;
+            rewrite <- H17 in M0; simpl in M0.
+        ** destruct M0 as [M0 | M0]; try contradiction.
+           rewrite <- M0 in H2. simpl in H2. inversion H2.
+        ** destruct M0 as [M0 | [M0 | M0]]; try contradiction.
+           *** rewrite <- M0 in H2. simpl in H2. inversion H2.
+           *** eapply option_I_to_O_helper; eauto.
+               rewrite <- M0 in J.
+               rewrite <- M0. simpl.               
+               exact J.
+    + not_or ctr ctr0 H9.
+    + not_or ctr ctr0 H9.
+    + ctr_case_analysis ctr ctr0. inversion_event Ev. find_contradiction M.
+    + find_contradiction M.
+  - insert_consistent s Ss.
+    destruct_deleted D.
+    insert_consistent s' St.
+    induction St; subst s'.
+    + inversion_event Ev. find_contradiction_del M.
+    + inversion_event Ev. find_contradiction_del M.
+    + not_or ctr ctr0 H9.
+    + not_or ctr ctr0 H9.
+    + ctr_case_analysis ctr ctr0.
+      execute_own ctr H10.
+      case_analysis H10.
+      * unfold option_derivative in Exec. simpl in Exec.
+        rewrite H0 in Exec. inversion Exec.
+      * case_analysis H13.
+        ** case_analysis H14.
+           *** unfold option_derivative in Exec. simpl in Exec.
+               rewrite H0, H10, H12 in Exec. inversion Exec.
+           *** case_analysis H15.
+        ** case_analysis H15.
+           *** unfold option_derivative in Exec. simpl in Exec.
+               rewrite H0, H10, H12 in Exec. inversion Exec.
+           *** case_analysis H15.
+    + find_contradiction_del M.
+Qed.
+
+Print option_I_to_O.
+
+
+(* The issuer does not have a choice! *)
+Proposition I_does_not_have_a_choice :
+  forall s1 s2 s t period I O sc ctr c_id dsc_id,
+    consistent_state s1 ->
+    ctr = finctr c_id dsc_id (option_derivative t period) I O O sc ->
+    O <> 0 ->
+    O <> I -> 
+    joins_in_s O ctr s1 s2 s t ->
+    forall gen_ctr, generates ctr gen_ctr s I O -> ctr_owner gen_ctr <> I.
+Proof.
+  intros.
+  destruct H3 as [s' [Ss1 [Ss2 [E | D]]]].
+  - destruct_executed E.
+    insert_consistent s Ss1.
+    induction St; subst s'.
+    + inversion_event Ev. find_contradiction M.
+    + ctr_case_analysis ctr ctr0.
+      execute_own ctr H11.
+      destruct_generates H4.
+      simpl in Exec.
+      case_analysis H11.
+      case_analysis H14. rewrite H0, H4 in *.
+      * case_analysis H15.
+        case_analysis H16; rewrite H13, H14 in *; subst res; simpl in *.
+        ** destruct M0 as [M0 | M0]; try contradiction.
+           subst gen_ctr. simpl. trivial.
+        ** destruct M0 as [M0 | [M0 | M0]]; try contradiction; try subst gen_ctr; simpl; trivial.
+      * case_analysis H15.
+        case_analysis H16; rewrite H13, H14 in *; subst res; simpl in *.
+        ** destruct M0 as [M0 | M0]; try contradiction.
+           subst gen_ctr. simpl. trivial.
+        ** destruct M0 as [M0 | [M0 | M0]]; try contradiction; try subst gen_ctr; simpl; trivial.
+    + not_or ctr ctr0 H8.
+    + not_or ctr ctr0 H8.
+    + ctr_case_analysis ctr ctr0. inversion_event Ev. find_contradiction M.
+    + find_contradiction M.
+  - destruct_deleted D.
+    insert_consistent s Ss1.
+    induction St; subst s'.
+    + inversion_event Ev. find_contradiction_del M.
+    + inversion_event Ev. find_contradiction_del M.
+    + not_or ctr ctr0 H8.
+    + not_or ctr ctr0 H8.
+    + ctr_case_analysis ctr ctr0.
+      execute_own ctr H9.
+      destruct_generates H4.
+      simpl in Exec.
+      case_analysis H9.
+      case_analysis H12; rewrite H0, H4 in *.
+      * case_analysis H13.
+        case_analysis H14; rewrite H11, H12 in *; try inversion H9.
+      * case_analysis H13.
+        case_analysis H14; rewrite H11, H12 in H9; try inversion H9.
+    + find_contradiction_del M.
+Qed.
+
+
+Print I_does_not_have_a_choice.
+
+(* The issuer's rights: the issuer is paid if the owner joins the generated Or *)
+Lemma option_O_to_I_helper:
+  forall s1 s2 t I O sc ctr c_id dsc_id,
+    consistent_state s1 ->
+    ctr = finctr c_id dsc_id (Or (Give (One USD)) (Give (One EUR))) I O O sc ->
+    joins O ctr s1 s2 t ->
+    O <> 0 ->
+    exists tr,
+      In tr (m_ledger s2) /\
+      tr_ctr_id tr = c_id /\
+      tr_from tr = O /\
+      tr_to tr = I /\
+      tr_amount tr = sc.
+Proof.
+  intros.
+  destruct_join H1.
+  - insert_consistent s Ss.
+    insert_consistent s' St.
+    induction St; subst s'.
+    + inversion_event Ev. find_contradiction M.
+    + ctr_case_analysis ctr ctr0. subst ctr. simpl in H7. contradiction.
+    + ctr_case_analysis ctr ctr0.
+      rewrite H0 in H10, H7. simpl in H7. inversion H7.
+      unfold exec_prim_ctr_in_state_with_owner in H10.
+      subst c1 c2. simpl in H10. inversion H10.
+      eexists. split.
+      * eapply steps_does_not_remove_transactions; eauto.
+        subst ledger'. simpl. left. trivial.
+      * repeat split; trivial. resolve_owner H5.
+    + ctr_case_analysis ctr ctr0.
+      rewrite H0 in H10, H7. simpl in H7. inversion H7.
+      unfold exec_prim_ctr_in_state_with_owner in H10.
+      subst c1 c2. simpl in H10. inversion H10.
+      eexists. split.
+      * eapply steps_does_not_remove_transactions; eauto.
+        subst ledger'. simpl. left. trivial.
+      * repeat split; trivial. resolve_owner H5.
+    + ctr_case_analysis ctr ctr0. execute_own ctr H8. inversion H8.
+    + find_contradiction M.
+  - insert_consistent s Ss.
+    insert_consistent s' St.
+    induction St; subst s'.
+    + inversion_event Ev. find_contradiction_del M.
+    + ctr_case_analysis ctr ctr0. subst ctr. simpl in H7. contradiction.
+    + simpl in Ev. inversion_event Ev. find_contradiction_del M.
+    + simpl in Ev. inversion_event Ev. find_contradiction_del M.
+    + ctr_case_analysis ctr ctr0. execute_own ctr H8. inversion H8.
+    + find_contradiction_del M.
+Qed.
+
+Proposition option_O_to_I:
+  forall s1 s2 t T gen_ctr period I O sc ctr c_id dsc_id,
+    consistent_state s1 ->
+    ctr = finctr c_id dsc_id (option_derivative t period) I O O sc ->
+    joins_generated O ctr gen_ctr s1 s2 t T ->
+    (ctr_primitive gen_ctr) = Or (Give (One USD)) (Give (One EUR)) ->
+    O <> 0 ->
+    exists tr,
+      In tr (m_ledger s2) /\
+      tr_ctr_id tr = (ctr_id gen_ctr) /\
+      tr_from tr = O /\
+      tr_to tr = I /\
+      tr_amount tr = sc.
+Proof.
+  intros.
+  destruct_join_gen H1.
+  - insert_consistent s Ss.
+    insert_consistent s' St.
+    induction St; subst s'.
+    + inversion_event Ev. find_contradiction M.
+    + ctr_case_analysis ctr ctr0.
+      execute_own ctr H11.
+      case_analysis H11.
+      case_analysis H14.
+      * case_analysis H15.
+        case_analysis H16.
+        ** subst t. apply ltb_sound_true in H14. contradict H14. omega.
+        ** simpl in Exec. rewrite H0, H11, H13, H14 in Exec.
+           inversion Exec. subst res. simpl in *.
+           destruct M0 as [M0 | [M0 | M0]]; try contradiction.
+           *** eapply option_O_to_I_helper; eauto.
+               rewrite <- M0 in J. rewrite <- M0.
+               exact J.
+           *** rewrite <- M0 in H2. simpl in H2. inversion H2.
+      * case_analysis H15.
+        case_analysis H16.
+        ** subst t. apply ltb_sound_true in H14. contradict H14. omega.
+        ** simpl in Exec. rewrite H0, H11, H13, H14 in Exec.
+           inversion Exec. subst res. simpl in *.
+           destruct M0 as [M0 | [M0 | M0]]; try contradiction;
+             rewrite <- M0 in H2; simpl in H2; inversion H2.
+    + not_or ctr ctr0 H8.
+    + not_or ctr ctr0 H8.
+    + ctr_case_analysis ctr ctr0. inversion_event Ev. find_contradiction M.
+    + find_contradiction M.
+  - insert_consistent s Ss.
+    destruct_deleted D.
+    insert_consistent s' St.
+    induction St; subst s'.
+    + inversion_event Ev. find_contradiction_del M.
+    + inversion_event Ev. find_contradiction_del M.
+    + not_or ctr ctr0 H8.
+    + not_or ctr ctr0 H8.
+    + ctr_case_analysis ctr ctr0.
+      execute_own ctr H9.
+      case_analysis H9.
+      * simpl in Exec. rewrite H0 in Exec. inversion Exec.
+      * case_analysis H12.
+        ** case_analysis H13; try case_analysis H14.
+           apply ltb_sound_true in H11.
+           apply Nat.lt_asymm in H11.
+           contradict H11. eapply infinite.
+        ** case_analysis H13; try case_analysis H14.
+           apply ltb_sound_true in H11.
+           apply Nat.lt_asymm in H11.
+           contradict H11. eapply infinite.
+    + find_contradiction_del M.
+Qed.
+
+Print option_O_to_I.
